Dafny/examples/generalInstructions.i.dfy
@@ -4,6 +4,7 @@ include "../types.dfy"
 include "../memory.dfy"
 include "../Operations/binaryOperations.i.dfy"
 include "../Operations/conversionOperations.i.dfy"
+include "../Operations/bitwiseBinaryOperations.i.dfy"
 
 module general_instructions {
     import opened LLVM_def
@@ -12,6 +13,7 @@ module general_instructions {
     import opened memory
     import opened binary_operations_i
     import opened conversion_operations_i
+    import opened bitwise_binary_operations_i
 
 function method{:opaque}lvm_code_Add(dst:lvm_operand_opr, size:nat, src1:lvm_operand_opr,src2:lvm_operand_opr):lvm_code
 
@@ -71,6 +73,8 @@ lemma lvm_lemma_Add(lvm_b0:lvm_codes, lvm_s0:lvm_state, lvm_sN:lvm_state,
     assert evalCode_lax(lvm_Block(lvm_b0), lvm_s0, lvm_sN,dst);
     assert lvm_s0.ok;
     assert eval_code(lvm_Block(lvm_b0), lvm_s0, lvm_sN,dst);
+    assert evalBlock(lvm_Block(lvm_b0).block, lvm_s0, lvm_sN,dst);
+    assert exists r' :: (evalCode(lvm_b0.hd, lvm_s0, r',dst));
 
     ghost var lvm_ltmp1, lvm_cM:lvm_code, lvm_ltmp2 := lvm_lemma_block(lvm_b0, lvm_s0, lvm_sN,dst);
     lvm_sM := lvm_ltmp1;
@@ -163,8 +167,9 @@ lemma lvm_lemma_Ret(lvm_b0:lvm_codes, lvm_s0:lvm_state, lvm_sN:lvm_state,dst:lvm
 //   
   ensures  lvm_ensure(lvm_b0, lvm_bM, lvm_s0, lvm_sM, lvm_sN,dst)
   ensures  lvm_get_ok(lvm_sM)
-  ensures lvm_s0 == lvm_sM
+  ensures  OperandContents(lvm_s0,op1).Void? ==> lvm_s0 == lvm_sM
   ensures  lvm_state_eq(lvm_sM,  lvm_s0)
+  ensures lvm_bM == lvm_b0.tl;
 {
   reveal_lvm_RET();
   reveal_ValidData();
@@ -177,13 +182,113 @@ lemma lvm_lemma_Ret(lvm_b0:lvm_codes, lvm_s0:lvm_state, lvm_sN:lvm_state,dst:lvm
   lvm_sM := lvm_ltmp1;
   lvm_bM := lvm_ltmp2;
 //   var lvm_b1:lvm_codes := lvm_get_block(lvm_cM);
-  assert lvm_sM.ok;
+  // assert lvm_sM.ok;
   assert lvm_b0.tl == lvm_bM;
 
   assert ValidState(lvm_sM);
-  assert evalCode_lax(lvm_cM, lvm_s0, lvm_sM,dst);
+  assert evalCode(lvm_cM, lvm_s0, lvm_sM,dst);
   reveal_evalCodeOpaque();
 }
+
+// lemma lvm_lemma_Ret(lvm_b0:lvm_codes, lvm_s0:lvm_state, lvm_sN:lvm_state,dst:lvm_operand_opr,op1:lvm_operand_opr)
+//   returns (lvm_bM:lvm_codes, lvm_sM:lvm_state)
+  
+//   requires exists a :: lvm_require(lvm_b0, lvm_RET(dst,op1), lvm_s0, lvm_sN,a)
+//   requires lvm_is_dst_opr(dst, lvm_s0)
+//   requires lvm_is_src_opr(op1, lvm_s0)
+//   requires lvm_get_ok(lvm_s0)
+//   requires ValidOperand(lvm_s0,dst);
+
+//   requires ValidOperand(lvm_s0,op1);
+
+// //   
+//   ensures  lvm_ensure(lvm_b0, lvm_bM, lvm_s0, lvm_sM, lvm_sN,dst)
+//   ensures  lvm_get_ok(lvm_sM)
+//   // ensures lvm_s0 == lvm_sM
+//   // ensures  lvm_state_eq(lvm_sM,  lvm_s0)
+// {
+//   reveal_lvm_RET();
+//   reveal_ValidData();
+//   reveal_evalCodeOpaque();
+//   reveal_eval_code();
+
+//   assert lvm_b0.hd.Ins? && lvm_b0.hd.ins.RET?;
+//   // dst :| evalBlock(lvm_b0, lvm_s0, lvm_sN,dst);
+//   // assert evalBlock(lvm_b0, lvm_s0, lvm_sN,dst);
+//       // assert eval_code(lvm_Block(lvm_b0), lvm_s0, lvm_sN,dst);
+
+//   // assert ValidInstruction(lvm_s0, lvm_b0.hd.ins);
+//   // assert exists r' :: ValidData(r',OperandContents(lvm_s0,lvm_b0.hd.ins.val));
+//   // assert exists r' :: (evalCode(lvm_b0.hd, lvm_s0, r',dst)); //&& evalBlock(lvm_b0.tl, r', lvm_sN,dst));
+//   // assert if lvm_b0.hd.ins.val.Void? then evalRet(lvm_s0, dst, lvm_b0.hd.ins.val, lvm_s0) 
+//   // else evalUpdate(lvm_s0, dst, lvm_b0.hd.ins.val, lvm_s0);
+//     // && OperandContents(lvm_s0, dst) == OperandContents(r', dst));
+          
+//   // assert exists r' :: (evalIns(lvm_b0.hd.ins, lvm_s0, r',dst));
+
+//   // assert evalBlock(lvm_b0, lvm_s0, lvm_sN,dst);
+
+//   // var r :| (evalIns(lvm_b0.hd.ins, lvm_s0, r,dst));
+//   // assert eval_code(Block(lvm_b0), lvm_s0, lvm_sN,dst);
+
+//   // assert dst == op1;
+
+//   ghost var lvm_ltmp1, lvm_cM:lvm_code, lvm_ltmp2 := lvm_lemma_block(lvm_b0, lvm_s0, lvm_sN,dst);
+//   lvm_sM := lvm_ltmp1;
+//   lvm_bM := lvm_ltmp2;
+// //   var lvm_b1:lvm_codes := lvm_get_block(lvm_cM);
+//   assert lvm_sM.ok;
+//   assert lvm_b0.tl == lvm_bM;
+
+//   assert ValidState(lvm_sM);
+//   assert evalCode_lax(lvm_cM, lvm_s0, lvm_sM,dst);
+//   reveal_evalCodeOpaque();
+// }
+
+
+
+// lemma lvm_lemma_Ret(lvm_b0:lvm_codes, lvm_s0:lvm_state, lvm_sN:lvm_state, op1:lvm_operand_opr)
+//   returns (lvm_bM:lvm_codes, lvm_sM:lvm_state, lvm_ret:lvm_operand_opr)
+  
+//   requires lvm_require(lvm_b0, lvm_RET(op1), lvm_s0, lvm_sN,op1)
+//   // requires lvm_is_dst_opr(lvm_ret, lvm_s0)
+//   requires lvm_is_src_opr(op1, lvm_s0)
+//   requires lvm_get_ok(lvm_s0)
+
+//   requires ValidOperand(lvm_s0,op1);
+
+// //   
+//   ensures  lvm_ensure(lvm_b0, lvm_bM, lvm_s0, lvm_sM, lvm_sN,lvm_ret)
+//   ensures  lvm_get_ok(lvm_sM)
+//   // ensures  lvm_s0 == lvm_sM
+//   // ensures ValidOperand(lvm_sM,op1);
+//   // ensures ValidOperand(lvm_sM,lvm_ret);
+//   // ensures OperandContents(lvm_sM,op1) ==  OperandContents(lvm_sM,lvm_ret);
+//   // ensures  lvm_state_eq(lvm_sM,  lvm_s0)
+// {
+//   reveal_lvm_RET();
+//   reveal_ValidData();
+//   reveal_evalCodeOpaque();
+//   reveal_eval_code();
+  
+//   lvm_ret :| lvm_require(lvm_b0, lvm_RET(op1), lvm_s0, lvm_sN,lvm_ret);
+//   assert evalBlock(lvm_b0, lvm_s0, lvm_sN,lvm_ret);
+//   assert ValidInstruction(lvm_s0, lvm_RET(op1).ins);
+
+//   ghost var lvm_ltmp1, lvm_cM:lvm_code, lvm_ltmp2 := lvm_lemma_block(lvm_b0, lvm_s0, lvm_sN,lvm_ret);
+//   lvm_sM := lvm_ltmp1;
+//   lvm_bM := lvm_ltmp2;
+// //   var lvm_b1:lvm_codes := lvm_get_block(lvm_cM);
+//   assert lvm_sM.ok;
+//   assert lvm_b0.tl == lvm_bM;
+
+//   assert ValidState(lvm_sM);
+//   // assert ValidOperand(lvm_sM,op1);
+//   // assert ValidOperand(lvm_sM,lvm_ret);
+//   // assert OperandContents(lvm_sM,op1) ==  OperandContents(lvm_sM,lvm_ret);
+//   assert evalCode_lax(lvm_cM, lvm_s0, lvm_sM,lvm_ret);
+//   reveal_evalCodeOpaque();
+// }
 
 function method{:opaque} lvm_LOAD(dst:lvm_operand_opr,s:MemState,t:bitWidth,op1:lvm_operand_opr):lvm_code
 {
@@ -400,6 +505,114 @@ lemma lvm_lemma_Sext(lvm_b0:lvm_codes, lvm_s0:lvm_state, lvm_sN:lvm_state,
   reveal_evalCodeOpaque();
 }
 
+function method{:opaque} lvm_code_SHL(dst:lvm_operand_opr,src:lvm_operand_opr,shiftAmt:lvm_operand_opr):(out:lvm_code)
+    ensures out.Ins?;
+{
+    reveal_IntFits();
+    Ins(SHL(dst,src,shiftAmt))
+}
+
+lemma lvm_lemma_Shl(lvm_b0:lvm_codes, lvm_s0:lvm_state, lvm_sN:lvm_state, 
+            dst:lvm_operand_opr, src:lvm_operand_opr,shiftAmt:lvm_operand_opr)
+  returns (lvm_bM:lvm_codes, lvm_sM:lvm_state)
+
+  requires lvm_require(lvm_b0, lvm_code_SHL(dst,src,shiftAmt), lvm_s0, lvm_sN,dst)
+  requires lvm_is_dst_opr(dst, lvm_s0)
+  requires lvm_is_src_opr(src, lvm_s0)
+  requires lvm_get_ok(lvm_s0)
+
+// is valid ins
+  requires ValidOperand(lvm_s0,src);
+  requires ValidOperand(lvm_s0,dst);
+  requires ValidOperand(lvm_s0,shiftAmt);
+
+  requires OperandContents(lvm_s0,src).Int?;
+  requires OperandContents(lvm_s0,dst).Int?;
+  requires OperandContents(lvm_s0,shiftAmt).Int?;
+  requires OperandContents(lvm_s0,src).itype.size*8 > OperandContents(lvm_s0,shiftAmt).val
+  requires OperandContents(lvm_s0,shiftAmt).val > 0
+  requires OperandContents(lvm_s0,dst).itype.signed == OperandContents(lvm_s0,src).itype.signed
+// //   
+  ensures  lvm_ensure(lvm_b0, lvm_bM, lvm_s0, lvm_sM, lvm_sN,dst)
+  ensures  lvm_get_ok(lvm_sM)
+  ensures  ValidOperand(lvm_sM,dst)
+  ensures  ValidOperand(lvm_sM,src)
+
+  ensures  OperandContents(lvm_sM,dst).Int?;
+  ensures  OperandContents(lvm_sM,src).Int?;
+
+  ensures OperandContents(lvm_sM,dst).itype.size == OperandContents(lvm_sM,src).itype.size 
+  ensures OperandContents(lvm_sM,dst).itype.signed == OperandContents(lvm_sM,src).itype.signed
+  ensures OperandContents(lvm_sM, dst) == evalSHL(OperandContents(lvm_s0,src),OperandContents(lvm_s0,shiftAmt));
+  ensures  lvm_state_eq(lvm_sM, lvm_update_ok(lvm_sM, lvm_update_all( lvm_sM, lvm_s0)))
+
+{
+    reveal_lvm_code_SHL();
+    reveal_evalCodeOpaque();
+    reveal_eval_code();
+    assert lvm_code_SHL(dst,src,shiftAmt).Ins?;
+
+    assert ValidInstruction(lvm_s0, lvm_code_SHL(dst,src,shiftAmt).ins);
+
+    ghost var lvm_ltmp1, lvm_cM:lvm_code, lvm_ltmp2 := lvm_lemma_block(lvm_b0, lvm_s0, lvm_sN,dst);
+    lvm_sM := lvm_ltmp1;
+    lvm_bM := lvm_ltmp2;
+    assert ValidState(lvm_s0);
+    assert ValidState(lvm_sM);
+  
+    assert lvm_sM.ok;
+    assert lvm_b0.tl == lvm_bM;
+
+    assert ValidState(lvm_sM);
+    assert evalCode_lax(lvm_cM, lvm_s0, lvm_sM,dst);
+    reveal_evalCodeOpaque();
+}
+
+
+function method{:opaque} lvm_code_Empty():lvm_code
+{   
+    lvm_Block(lvm_CNil())
+}       
+
+lemma lvm_lemma_Empty(lvm_b0:lvm_codes, lvm_s0:lvm_state, lvm_sN:lvm_state,o:operand)
+  returns (lvm_bM:lvm_codes, lvm_sM:lvm_state)
+  requires lvm_require(lvm_b0, lvm_code_Empty(), lvm_s0, lvm_sN,o)
+  requires lvm_get_ok(lvm_s0)
+  ensures  lvm_ensure(lvm_b0, lvm_bM, lvm_s0, lvm_sM, lvm_sN,o)
+  ensures  lvm_get_ok(lvm_sM) // ValidState(sM)
+  ensures  lvm_state_eq(lvm_sM, lvm_s0)
+  ensures  lvm_state_eq(lvm_sM, lvm_update_mem( lvm_sM, lvm_update_ok(lvm_sM, lvm_sM)))
+  ensures  forall s2 :: evalCode(lvm_b0.hd, lvm_s0, s2,o) ==> s2.ok 
+{
+    reveal_lvm_code_Empty();
+    reveal_eval_code();
+    reveal_evalCodeOpaque();
+
+    var lvm_old_s:lvm_state := lvm_s0;
+
+    assert lvm_s0.ok;
+    assert lvm_code_Empty() == Block(CNil);
+    assert lvm_b0.hd == lvm_code_Empty();
+    assert !lvm_b0.CNil?;
+    assert lvm_code_Empty().block.CNil?;
+    assert lvm_b0.hd.Block?;
+    assert lvm_get_block(lvm_b0.hd).CNil?;
+    assert evalBlock(lvm_get_block(lvm_b0.hd),lvm_s0, lvm_s0,o);
+    assert forall r :: r == lvm_s0 ==> eval_code(lvm_b0.hd,lvm_s0,r,o);
+    assert evalCode_lax(Block(lvm_b0), lvm_s0, lvm_sN, o);
+
+    assert evalBlock(lvm_b0, lvm_s0, lvm_sN,o) ==> exists r' :: evalCode(lvm_b0.hd, lvm_s0, r',o) && evalBlock(lvm_b0.tl, r', lvm_sN,o);
+    assert exists r' :: if evalCode(lvm_b0.hd, lvm_s0, r',o) then true else true;
+
+    // lvm_sM := lvm_lemma_empty(lvm_s0,lvm_sN);
+    ghost var lvm_ltmp1, lvm_cM:lvm_code, lvm_ltmp2 := lvm_lemma_block(lvm_b0, lvm_s0, lvm_sN,o);
+    lvm_sM := lvm_ltmp1;
+    lvm_bM := lvm_ltmp2;
+    var lvm_b1:lvm_codes := lvm_get_block(lvm_cM);
+    // assert evalCode_lax(lvm_Block(lvm_CNil()), lvm_s0, lvm_sM, o);
+
+    lvm_sM := lvm_lemma_empty(lvm_s0, lvm_sM);
+}
 
 
 }
