Dafny/examples/simple.i.dfy
@@ -15,51 +15,7 @@ module simple_functions {
     import opened binary_operations_i
 
 
-function method{:opaque} lvm_code_Empty():lvm_code
-{   
-    lvm_Block(lvm_CNil())
-}       
 
-lemma lvm_lemma_Empty_Test(lvm_b0:lvm_codes, lvm_s0:lvm_state, lvm_sN:lvm_state, src:lvm_operand_opr,o:operand)
-  returns (lvm_bM:lvm_codes, lvm_sM:lvm_state)
-  requires lvm_require(lvm_b0, lvm_code_Empty(), lvm_s0, lvm_sN,o)
-  requires lvm_is_src_opr(src, lvm_s0)
-  requires lvm_get_ok(lvm_s0)
-  ensures  lvm_ensure(lvm_b0, lvm_bM, lvm_s0, lvm_sM, lvm_sN,o)
-  ensures  lvm_get_ok(lvm_sM) // ValidState(sM)
-  ensures  lvm_state_eq(lvm_sM, lvm_s0)
-  ensures  lvm_state_eq(lvm_sM, lvm_update_mem( lvm_sM, lvm_update_ok(lvm_sM, lvm_sM)))
-  ensures  forall s2 :: evalCode(lvm_b0.hd, lvm_s0, s2,o) ==> s2.ok
-{
-    reveal_lvm_code_Empty();
-    reveal_eval_code();
-    reveal_evalCodeOpaque();
-
-    var lvm_old_s:lvm_state := lvm_s0;
-
-    assert lvm_s0.ok;
-    assert lvm_code_Empty() == Block(CNil);
-    assert lvm_b0.hd == lvm_code_Empty();
-    assert !lvm_b0.CNil?;
-    assert lvm_code_Empty().block.CNil?;
-    assert lvm_b0.hd.Block?;
-    assert lvm_get_block(lvm_b0.hd).CNil?;
-    assert evalBlock(lvm_get_block(lvm_b0.hd),lvm_s0, lvm_s0,o);
-    assert forall r :: r == lvm_s0 ==> eval_code(lvm_b0.hd,lvm_s0,r,o);
-    assert evalCode_lax(Block(lvm_b0), lvm_s0, lvm_sN, o);
-
-    assert evalBlock(lvm_b0, lvm_s0, lvm_sN,o) ==> exists r' :: evalCode(lvm_b0.hd, lvm_s0, r',o) && evalBlock(lvm_b0.tl, r', lvm_sN,o);
-    assert exists r' :: if evalCode(lvm_b0.hd, lvm_s0, r',o) then true else true;
-
-    // lvm_sM := lvm_lemma_empty(lvm_s0,lvm_sN);
-    ghost var lvm_ltmp1, lvm_cM:lvm_code, lvm_ltmp2 := lvm_lemma_block(lvm_b0, lvm_s0, lvm_sN,o);
-    lvm_sM := lvm_ltmp1;
-    lvm_bM := lvm_ltmp2;
-    var lvm_b1:lvm_codes := lvm_get_block(lvm_cM);
-    // assert evalCode_lax(lvm_Block(lvm_CNil()), lvm_s0, lvm_sM, o);
-
-    lvm_sM := lvm_lemma_empty(lvm_s0, lvm_sM);
-}
 
 
 ////
@@ -233,7 +189,7 @@ lemma lvm_lemma_Add_Multiple(lvm_b0:lvm_codes, lvm_s0:lvm_state, lvm_sN:lvm_stat
     
     ghost var lvm_b4, lvm_s4 := lvm_lemma_Ret(lvm_b3, lvm_s3, lvm_sM, dst, D(Void));
     assert lvm_b4.CNil?;
-
+    assert eval_code(lvm_Block(lvm_b4), lvm_s4, lvm_sM,dst);
     lvm_sM := lvm_lemma_empty(lvm_s4,lvm_sM);
     assert   OperandContents(lvm_sM, dst).val  == step2.val;
 
